add: priority queue add method, not finished

source/PriorityQueue.dfy
@@ -10,6 +10,12 @@ class {:autocontracts} PriorityQueue<T> {
 	{
 		// The priorities follow an order
 		true
+		// isOrdered()
+	}
+
+	predicate isOrdered() 
+	{
+		forall i, j :: 0 <= i < j < size() ==> sequence[i].0 <= sequence[j].0
 	}
 
 	function method size() : nat
@@ -22,9 +28,25 @@ class {:autocontracts} PriorityQueue<T> {
 		|sequence| == 0
 	}
 	
-	method add(element : T, priority : nat)
+	method add(priority : nat, element : T)
+	requires isOrdered()
+	ensures isOrdered()
+	ensures size() == old(size()) + 1
 	{
-
+		var i := 0;
+		while i < size()
+		invariant 0 <= i <= size()
+		invariant isOrdered()
+		decreases size() - i
+		{
+			if priority < sequence[i].0
+			{
+				sequence :=  sequence[..i] + [(priority, element)] + sequence[i..];
+				return;
+			}
+			i := i + 1;
+		}
+    	sequence :=  sequence + [(priority, element)];
 	}
 
 	method pop()
